rules/rules_isect_member_equality.v
@@ -1,0 +1,345 @@
+(*
+
+  Copyright 2014 Cornell University
+  Copyright 2015 Cornell University
+  Copyright 2016 Cornell University
+  Copyright 2017 Cornell University
+
+  This file is part of VPrl (the Verified Nuprl project).
+
+  VPrl is free software: you can redistribute it and/or modify
+  it under the terms of the GNU General Public License as published by
+  the Free Software Foundation, either version 3 of the License, or
+  (at your option) any later version.
+
+  VPrl is distributed in the hope that it will be useful,
+  but WITHOUT ANY WARRANTY; without even the implied warranty of
+  MERCHANTABILITY or FITNESS FOR A PARTICULAR PURPOSE.  See the
+  GNU General Public License for more details.
+
+  You should have received a copy of the GNU General Public License
+  along with VPrl.  If not, see <http://www.gnu.org/licenses/>.
+
+
+  Websites: http://nuprl.org/html/verification/
+            http://nuprl.org/html/Nuprl2Coq
+            https://github.com/vrahli/NuprlInCoq
+
+  Authors: Abhishek Anand & Vincent Rahli
+
+*)
+
+
+Require Export sequents2.
+Require Export sequents_lib.
+Require Export sequents_tacs.
+Require Export sequents_tacs2.
+Require Export sequents_equality.
+Require Export rules_useful.
+Require Export per_props_equality.
+Require Export per_props_isect.
+Require Export rules_tyfam.
+Require Export rules_tyfam2.
+Require Export subst_tacs_aeq.
+Require Export cequiv_tacs.
+Require Export lsubstc_weak.
+Require Export rules_elimination.
+
+
+Hint Rewrite @nh_vars_hyps_app : slow.
+Hint Rewrite @nh_vars_hyps_snoc : slow.
+
+
+(**
+
+<<
+
+   H |- t1 = t2 in isect(x:A;B)
+
+     By isect_memberEquality lvl(i) z ()
+
+     H z : A |- t1 = t2 in B[x\z]
+     H |- A = A in Type(i)
+>>
+ *)
+
+Definition rule_isect_member_equality_concl {o} (H : @bhyps o) t1 t2 A x B :=
+  mk_baresequent H (mk_conclax (mk_equality t1 t2 (mk_isect A x B))).
+
+Definition rule_isect_member_equality_hyp1 {o} (H : @bhyps o) z A t1 t2 B x e1 :=
+  mk_baresequent
+    (snoc H (mk_hyp z A))
+    (mk_concl (mk_equality t1 t2 (subst B x (mk_var z))) e1).
+
+Definition rule_isect_member_equality_hyp2 {o} (H : @bhyps o) A i e2 :=
+  mk_baresequent H (mk_concl (mk_equality A A (mk_uni i)) e2).
+
+Definition rule_isect_member_equality {o}
+           (A B t1 t2 e1 e2 : NTerm)
+           (x z : NVar)
+           (i : nat)
+           (H : @barehypotheses o) :=
+  mk_rule
+    (rule_isect_member_equality_concl H t1 t2 A x B)
+    [ rule_isect_member_equality_hyp1 H z A t1 t2 B x e1,
+      rule_isect_member_equality_hyp2 H A i e2 ]
+    [sarg_var z].
+
+Lemma rule_isect_member_equality_true3 {o} :
+  forall lib (A B t1 t2 e1 e2 : NTerm)
+         (x z : NVar)
+         (i   : nat)
+         (H   : @barehypotheses o),
+    rule_true3 lib (rule_isect_member_equality A B t1 t2 e1 e2 x z i H).
+Proof.
+  intros.
+  unfold rule_isect_member_equality, rule_true3, wf_bseq, closed_type_baresequent, closed_extract_baresequent; simpl.
+  intros.
+
+  (* We prove the well-formedness of things *)
+  destseq; allsimpl.
+  dLin_hyp; exrepnd.
+  rename Hyp into hyp1.
+  rename Hyp0 into hyp2.
+  destruct hyp1 as [ ws1 hyp1 ].
+  destruct hyp2 as [ ws2 hyp2 ].
+  destseq; allsimpl; proof_irr; GC.
+
+  match goal with
+  | [ |- sequent_true2 _ ?s ] => assert (wf_csequent s) as wfc
+  end.
+  {
+    clear hyp1 hyp2.
+    unfold wf_csequent, closed_type, closed_extract, wf_sequent, wf_concl; simpl.
+    prove_seq; eauto 3 with slow.
+  }
+  exists wfc.
+  unfold wf_csequent, wf_sequent, wf_concl in wfc; allsimpl; repnd; proof_irr; GC.
+
+  (* We prove some simple facts on our sequents *)
+  assert ((z <> x -> !LIn z (free_vars B))
+          # !LIn z (free_vars t1)
+          # !LIn z (free_vars t2)
+          # !LIn z (free_vars A)
+          # !LIn z (vars_hyps H)) as vhyps.
+
+  {
+    clear hyp1 hyp2.
+    dwfseq.
+    sp;
+      try (complete (pose proof (wfc1 z) as q; allrw in_remove_nvars;
+                     allrw in_single_iff; autodimp q hyp)).
+  }
+
+  destruct vhyps as [ nzB  vhyps ].
+  destruct vhyps as [ nzt1 vhyps ].
+  destruct vhyps as [ nzt2 vhyps ].
+  destruct vhyps as [ nzA nzH ].
+  (* done with proving these simple facts *)
+
+  (* we now start proving the sequent *)
+  vr_seq_true.
+
+  lsubst_tac.
+  allrw <- @member_equality_iff.
+  teq_and_eq (mk_isect A x B) t1 t2 s1 s2 H.
+
+  - apply tequality_isect; dands.
+
+    + vr_seq_true in hyp2.
+      pose proof (hyp2 s1 s2 eqh sim) as hyp2; exrepnd.
+      lsubst_tac.
+      apply equality_in_mkc_equality in hyp2; repnd.
+      apply equality_commutes2 in hyp0; auto.
+      apply equality_in_uni in hyp0; auto.
+
+    + introv eqa.
+
+      vr_seq_true in hyp1.
+      pose proof (hyp1 (snoc s1 (z,a)) (snoc s2 (z,a'))) as hyp1.
+      repeat (autodimp hyp1 xxx).
+
+      {
+        apply hyps_functionality_snoc2; simpl; auto.
+        introv equ sim'.
+
+        vr_seq_true in hyp2.
+        pose proof (hyp2 s1 s' eqh sim') as hyp2; exrepnd.
+        lsubst_tac.
+        apply equality_in_mkc_equality in hyp1; repnd.
+        apply equality_commutes2 in hyp0; auto.
+        apply equality_in_uni in hyp0; auto.
+      }
+
+      {
+        sim_snoc; dands; auto.
+      }
+
+      exrepnd.
+      lsubst_tac.
+      apply tequality_mkc_equality_sp in hyp0; repnd.
+      clear hyp0 hyp4.
+
+      assert (cover_vars (mk_var z) (snoc s1 (z, a))) as covz1.
+      { apply cover_vars_var; rw @dom_csub_snoc; simpl; apply in_snoc; tcsp. }
+
+      assert (cover_vars (mk_var z) (snoc s2 (z, a'))) as covz2.
+      { apply cover_vars_var; rw @dom_csub_snoc; simpl; apply in_snoc; tcsp. }
+
+      repeat (lsubstc_subst_aeq2;[]).
+      repeat (substc_lsubstc_vars3;[]).
+
+      revert c13 c14 hyp3.
+      lsubst_tac.
+      introv t.
+      repeat (lsubstc_snoc2;[]).
+      clear_irr.
+      auto.
+
+  - apply equality_in_isect2; dands.
+
+    + vr_seq_true in hyp2.
+      pose proof (hyp2 s1 s2 hf sim) as hyp2; exrepnd.
+      lsubst_tac.
+      apply equality_in_mkc_equality in hyp2; repnd.
+      apply equality_commutes2 in hyp0; auto.
+      apply equality_in_uni in hyp0; auto.
+      eapply tequality_trans;[eauto|]; apply tequality_sym; auto.
+
+    + introv eqa.
+
+      dands.
+
+      * vr_seq_true in hyp1.
+        pose proof (hyp1 (snoc s1 (z,a)) (snoc s2 (z,a'))) as hyp1.
+        repeat (autodimp hyp1 xxx).
+
+        {
+          apply hyps_functionality_snoc2; simpl; auto.
+          introv equ sim'.
+
+          vr_seq_true in hyp2.
+          pose proof (hyp2 s1 s' hf sim') as hyp2; exrepnd.
+          lsubst_tac.
+          apply equality_in_mkc_equality in hyp1; repnd.
+          apply equality_commutes2 in hyp0; auto.
+          apply equality_in_uni in hyp0; auto.
+        }
+
+        {
+          sim_snoc; dands; auto.
+        }
+
+        exrepnd.
+        lsubst_tac.
+
+        apply equality_in_mkc_equality in hyp1; repnd.
+        clear hyp1 hyp4.
+
+        apply equality_commutes4 in hyp0; auto.
+        clear hyp3.
+
+        assert (cover_vars (mk_var z) (snoc s1 (z, a))) as covz1.
+        { apply cover_vars_var; rw @dom_csub_snoc; simpl; apply in_snoc; tcsp. }
+
+        assert (cover_vars (mk_var z) (snoc s2 (z, a'))) as covz2.
+        { apply cover_vars_var; rw @dom_csub_snoc; simpl; apply in_snoc; tcsp. }
+
+        repeat (lsubstc_subst_aeq2;[]).
+        repeat (substc_lsubstc_vars3;[]).
+
+        revert c8 hyp0.
+        lsubst_tac.
+        introv t.
+        repeat (lsubstc_snoc2;[]).
+        clear_irr.
+        auto.
+
+      * vr_seq_true in hyp1.
+        pose proof (hyp1 (snoc s1 (z,a)) (snoc s1 (z,a'))) as hyp1.
+        repeat (autodimp hyp1 xxx).
+
+        {
+          apply hyps_functionality_snoc2; simpl; auto.
+          introv equ sim'.
+
+          vr_seq_true in hyp2.
+          pose proof (hyp2 s1 s' hf sim') as hyp2; exrepnd.
+          lsubst_tac.
+          apply equality_in_mkc_equality in hyp1; repnd.
+          apply equality_commutes2 in hyp0; auto.
+          apply equality_in_uni in hyp0; auto.
+        }
+
+        {
+          sim_snoc; dands; auto.
+          eapply similarity_refl; eauto.
+        }
+
+        exrepnd.
+        lsubst_tac.
+
+        apply tequality_mkc_equality_sp in hyp0; repnd.
+        clear hyp0 hyp4.
+
+        assert (cover_vars (mk_var z) (snoc s1 (z, a))) as covz1.
+        { apply cover_vars_var; rw @dom_csub_snoc; simpl; apply in_snoc; tcsp. }
+
+        assert (cover_vars (mk_var z) (snoc s1 (z, a'))) as covz2.
+        { apply cover_vars_var; rw @dom_csub_snoc; simpl; apply in_snoc; tcsp. }
+
+        repeat (lsubstc_subst_aeq2;[]).
+        repeat (substc_lsubstc_vars3;[]).
+
+        revert c8 c9 hyp3.
+        lsubst_tac.
+        introv t.
+        repeat (lsubstc_snoc2;[]).
+        clear_irr.
+        auto.
+Qed.
+
+Lemma rule_isect_member_equality_true_ext_lib {o} :
+  forall lib (A B t1 t2 e1 e2 : NTerm)
+         (x z : NVar)
+         (i   : nat)
+         (H   : @barehypotheses o),
+    rule_true_ext_lib lib (rule_isect_member_equality A B t1 t2 e1 e2 x z i H).
+Proof.
+  introv.
+  apply rule_true3_implies_rule_true_ext_lib.
+  introv.
+  apply rule_isect_member_equality_true3.
+Qed.
+
+Lemma rule_isect_member_equality_wf2 {o} :
+  forall (A B t1 t2 e1 e2 : NTerm)
+         (x z : NVar)
+         (i   : nat)
+         (H   : @barehypotheses o),
+    !LIn z (vars_hyps H)
+    -> wf_rule2 (rule_isect_member_equality A B t1 t2 e1 e2 x z i H).
+Proof.
+  introv nizH  wf j; allsimpl; repndors; subst; tcsp;
+    allunfold @wf_bseq; repnd; allsimpl; wfseq;
+      allrw @covered_isect; repnd; auto;
+        allrw <- @wf_isect_iff; repnd; auto.
+
+  - allrw @vswf_hypotheses_nil_eq.
+    allrw @wf_hypotheses_snoc.
+    dands; auto; simpl.
+    apply isprog_vars_iff_covered; dands; auto.
+
+  - apply wf_term_subst; eauto 2 with slow.
+
+  - apply covered_snoc_weak; auto.
+
+  - apply covered_snoc_weak; auto.
+
+  - apply covered_subst; auto.
+
+    + rewrite cons_snoc.
+      apply covered_snoc_weak; auto.
+
+    + apply covered_var; rw in_snoc; tcsp.
+Qed.
